complete mulzq proof, spec poly mul

code/mlkem/Hacl.MLkem.Poly.fst
@@ -9,133 +9,284 @@ module B = LowStar.Buffer
 module ST = FStar.HyperStack.ST
 module HS = FStar.HyperStack
 module S = Hacl.Spec.MLkem.Poly
+module Seq = Lib.Sequence
 module M = LowStar.Modifies
+module U32 = FStar.UInt32
 
+open FStar.Ghost
 open Lib.Buffer
 open Lib.IntTypes
 // open Lib.Loops
 
-val main: unit -> Stack UInt32.t (requires fun _ -> True) (ensures fun _ _ _ -> True)
-let main () = 0ul
-
 #reset-options "--z3rlimit 50 --fuel 0 --ifuel 0"
 
-let q: uint32 = u32 S.q
-let zq = x:uint32{ v x < v q /\ v x >= 0 }
+let n: size_t = size S.n
+let q32: uint32 = u32 S.q
+let q64: uint64 = u64 S.q
+let m: uint64 = u64 S.m
+let zq = x:uint32{v x < S.q}
+
+let zq_v (x:zq): S.zq = v x
 
 let lpoly deg = lbuffer zq deg
+let rq = lpoly n
 
-// Functions to convert from impl to spec for proofs
-let zq_to_s_zq (x:zq): S.zq =
-  v x
-let seq_int32_to_int (s:seq zq): (seq S.zq) =
-  init (Seq.length s) (fun i -> (zq_to_s_zq (Seq.index s i)))
-let poly_impl_to_spec #deg (p:lpoly deg) (h: HS.mem): GTot (S.lpoly (v deg)) =
-  seq_int32_to_int (as_seq h p)
-
-val poly_index:
-    #deg:size_t
-  -> p: lpoly deg
-  -> i:size_t
-  -> Stack (zq)
-    (requires fun h0 -> live h0 p)
-    (ensures fun h0 r h1 -> 
-      let res_zq = v r in 
-      let spec_zq = (S.poly_index (poly_impl_to_spec p h1) (v i)) in 
-      res_zq == spec_zq
-    )
-let poly_index #deg p i =
-  assert (v 0ul >= 0);
-  if 0ul <=. i && i <. deg then 
-    index p i
-  else u32 0
+val lpoly_v: #deg:size_t -> h:HS.mem -> p:lpoly deg -> GTot (S.lpoly (v deg))
+let lpoly_v #deg h p =
+  let s:lseq zq (v deg) = as_seq h p in
+  Seq.map zq_v s
+val rq_v: h:HS.mem -> p:rq -> GTot (S.lpoly (v n))
+let rq_v h p = lpoly_v #n h p
 
 val add_zq (a:zq) (b:zq): Pure (zq)
   (requires True)
-  (ensures fun r -> v r == (v a + v b) % (v q))
+  (ensures fun r -> zq_v r == S.add_zq (zq_v a) (zq_v b))
 let add_zq a b =
   // assert (v a + v b == v (a +. b)) ;
   let sum = a +. b in
-  let overflow_mask = lte_mask q sum in
+  let overflow_mask = lte_mask q32 sum in
   // assert (v overflow_mask == 0 \/ v overflow_mask == v 0xFFFFFFFFul) ;
-  let sub_value = logand overflow_mask q in
-  logand_lemma overflow_mask q ;
+  let sub_value = logand overflow_mask q32 in
+  logand_lemma overflow_mask q32 ;
   // assert (v sub_value == 0 \/ v sub_value == v q ) ;
   sum -. sub_value
 
+val mul_zq_lemma (a:zq) (b:zq): 
+  Lemma (requires True) (ensures (v (a *. b) == (v a * v b)))
+let mul_zq_lemma a b =
+  assert (v a < 3329);
+  // assert (v b < 3329);
+  assert (v a * v b < 3329 * 3329);
+  ()
+
+val error_increases_lemma (prodA:uint64{v prodA <= 3328 * 3328}) (prodB:uint64{v prodB <= 3328 * 3328}): 
+  Lemma 
+    (requires v prodA <= v prodB)
+    (ensures (
+      let quotA = (prodA *. m) >>. (32ul) in
+      let quotB = (prodB *. m) >>. (32ul) in
+      v quotA <= v quotB
+    ))
+let error_increases_lemma prodA prodB =
+  let quotA = (prodA *. m) >>. (32ul) in
+  let quotB = (prodB *. m) >>. (32ul) in
+  assert (v quotA <= v quotB);
+  ()
+  
+val quot_max_error_lemma (prod:uint64{v prod <= 3328 * 3328}): 
+  Lemma 
+    (requires True)
+    (ensures (
+      let quot = (prod *. m) >>. (32ul) in
+      v quot = (v prod / v q64) \/ v quot = ((v prod / v q64) - 1))
+    )
+let quot_max_error_lemma prod = 
+  assert (v prod < 3329 * 3329);
+  let maxProd = (q64 -. (u64 1)) *. (q64 -. (u64 1)) in
+  assert (v prod <= v maxProd);
+  error_increases_lemma prod maxProd;
+  ()
+
+    
+
+#reset-options "--z3rlimit 100 --fuel 0 --ifuel 0 --split_queries always"
+val mul_zq (a:zq) (b:zq): Pure (zq)
+  (requires True)
+  (ensures fun r -> zq_v r == S.mul_zq (zq_v a) (zq_v b))
+let mul_zq a b =
+  let prod = cast U64 SEC (a *. b) in
+  mul_zq_lemma a b ; // convinces fstar that there's no overflow
+  let quot = (prod *. m) >>. (32ul) in
+  assert (v a <= 3328 /\ v b <= 3328);
+  assert (v prod <= 3328 * 3328);
+  quot_max_error_lemma prod ;
+  assert (v quot = (v prod / v q64) \/ v quot = ((v prod / v q64) - 1)) ;
+  let rem = prod -. (quot *. q64) in
+  assert(v rem < 2 * v q64) ;
+  let overflow_mask = lte_mask q64 rem in
+  assert (v rem < v q64 \/ v overflow_mask = ones_v U64) ;
+  let sub_value = logand overflow_mask q64 in
+  // gt_mask_lemma rem q64 ;
+  logand_lemma overflow_mask q64 ;
+  let result = rem -. sub_value in
+  // assert (v result < v q64) ;
+  cast U32 SEC result
+
+#reset-options "--z3rlimit 50 --fuel 0 --ifuel 0"
+let empty #a: lseq a 0 = FStar.Seq.empty
+
+let cons #a #len (elem:a) (s:lseq a len): lseq a (len + 1) = FStar.Seq.cons elem s
+
+val slice_plus_one (#a:Type) (#len1 #len2:size_nat) (s1: lseq a len1) (s2: lseq a len2) (i: size_nat):
+  Lemma (requires (
+    i < len1 /\
+    i < len2 /\
+    Seq.equal (Seq.slice #_ #len1 s1 0 i) (Seq.slice #_ #len2 s2 0 i) /\
+    Seq.index #_ #len1 s1 i == Seq.index #_ #len2 s2 i))
+  (ensures Seq.equal (Seq.slice #_ #len1 s1 0 (i + 1)) (Seq.slice #_ #len2 s2 0 (i + 1)))
+let slice_plus_one #a #len1 #len2 s1 s2 i =
+  let x = Seq.index #_ #len1 s1 i in
+  let s1' = Seq.concat #_ #i #1 (Seq.slice #_ #len1 s1 0 i) (cons x empty) in
+  let s2' = Seq.concat #_ #i #1 (Seq.slice #_ #len2 s2 0 i) (cons x empty) in
+  assert (Seq.equal s1' (Seq.slice #_ #len1 s1 0 (i + 1)));
+  assert (Seq.equal s2' (Seq.slice #_ #len2 s2 0 (i + 1)))
 
 val add:
-  aDeg: size_t{v aDeg > 0}
-  -> a:lpoly aDeg
-  // -> bDeg: size_t{v bDeg = v aDeg}
-  -> b:lpoly aDeg
-  -> res:lpoly aDeg
+    #deg: size_t
+  -> a:lpoly deg
+  -> b:lpoly deg
+  -> res:lpoly deg
   -> Stack unit
   (requires fun h ->
-    live h a /\ 
-    live h b /\ 
-    live h res /\
+    live h a /\ live h b /\ live h res /\
+    disjoint a b /\ disjoint a res /\ disjoint b res
+  )
+  (ensures fun h0 _ h1 ->
+    live h1 a /\ 
+    live h1 b /\ 
+    live h1 res /\
     disjoint a b /\
     disjoint a res /\
-    disjoint b res
-  )
-  (ensures  fun h0 _ h1 ->
-    let spec_a = poly_impl_to_spec a h0 in
-    let spec_b = poly_impl_to_spec b h0 in
-    let spec_res = poly_impl_to_spec res h1 in 
+    disjoint b res /\
     modifies (loc res) h0 h1 /\
-    (Seq.equal spec_res (S.add spec_a spec_b))
-  )
+    Seq.equal (lpoly_v h1 res) (S.add (lpoly_v h0 a) (lpoly_v h0 b))
+   )
 
-// let seq_slice_equal (s1 s2: seq zq): Lemma 
-//   // (requires (Seq.equal (Seq.slice s1 (length s1)) (Seq.slice s2 (length s2))) /\ (Seq.length s1 == Seq.length s2) /\ (Seq.)) 
-//   (ensures Seq.equal s1 s2)
-
-let add aDeg a b res =
-  // push_frame ();
-  // let res0 = create aDeg (u32 0) in
+let add #deg a b res =
+  push_frame ();
   let h0 = ST.get () in
-  let inv h (i: nat{ i <= v aDeg}) =
-    let res_lowest = S.get_lowest_n (poly_impl_to_spec res h) i in
-    let first_i_a = S.get_lowest_n (poly_impl_to_spec a h) i in
-    let first_i_b = S.get_lowest_n (poly_impl_to_spec b h) i in
-    let add_a_b_lowest = S.add #i #i first_i_a first_i_b in
+  let spec_sum: erased _ = S.add (lpoly_v h0 a) (lpoly_v h0 b) in
+  let inv h (i:nat) =
+    live h a /\ live h b /\ live h res /\ modifies (loc res) h0 h /\
+    i <= v deg /\
+    Seq.equal (Seq.slice (lpoly_v h res) 0 i) (Seq.slice spec_sum 0 i) in
+  let body (i: U32.t{ 0 <= U32.v i /\ U32.v i < U32.v deg }):
+    Stack unit
+    (requires (fun h -> inv h (U32.v i)))
+    (ensures (fun h0 () h1 -> inv h0 (U32.v i) /\ inv h1 (U32.v i + 1)))
+    =
+      let h0 = ST.get () in
+      assert (Seq.equal (Seq.slice (lpoly_v h0 res) 0 (v i)) (Seq.slice spec_sum 0 (v i)));
+      let ai = a.(i) in
+      let bi = b.(i) in
+      let sum = add_zq ai bi in
+      res.(i) <- sum;
+      let h1 = ST.get () in
+      assert (Seq.equal (Seq.slice (lpoly_v h1 res) 0 (v i)) (Seq.slice spec_sum 0 (v i)));
+      assert (Seq.index (lpoly_v h1 res) (v i) == Seq.index spec_sum (v i));
+      slice_plus_one #_ #(v deg) #(v deg) (lpoly_v h1 res) spec_sum (v i)
+    in
+  Lib.Loops.for 0ul deg inv body;
+  pop_frame ()
 
-    // assert (Seq.length first_i_a == i);
-    // assert (Seq.length first_i_b == i);
-    // assert (Seq.length first_i_a == Seq.length first_i_b);
-
-    // assert (Seq.length res_lowest == Seq.length add_a_b_lowest);
-    // assert (Seq.length res_lowest == i);
-    // assert (S.poly_index res_lowest i == S.poly_index first_i_a i + S.poly_index first_i_b i);
-
-    // assume (S.poly_index res_lowest i == (S.poly_index first_i_a i) + (S.poly_index first_i_b i) % S.q);
-
-    // assume (Seq.equal (Seq.slice res_lowest 0 i) (Seq.slice add_a_b_lowest 0 i));
-    // assume (i = 0 \/ Seq.index res_lowest (i-1) == Seq.index add_a_b_lowest (i-1));
-    // assert (Seq.length res_lowest == i /\ Seq.length add_a_b_lowest == i);
-    // assume (i = 0 \/ Seq.equal (Seq.slice res_lowest 0 (i-1)) (Seq.slice add_a_b_lowest 0 (i-1)));
-    // assume (i = v aDeg \/ (Seq.index res_lowest i) = (Seq.index add_a_b_lowest i));
-    // assume (i = 0 \/ Seq.index res_lowest (i-1) == Seq.index add_a_b_lowest (i-1));
-    
-    assume (Seq.equal res_lowest add_a_b_lowest);
+val add_rq: 
+    a: rq 
+  -> b: rq 
+  -> res: rq 
+  -> Stack unit
+  (requires fun h ->
     live h a /\ live h b /\ live h res /\
-    disjoint a b /\ disjoint a res /\ disjoint b res /\
-    i <= v aDeg /\
-    (modifies (loc res) h0 h) /\
-    Seq.equal res_lowest add_a_b_lowest
-    
-    // res_lowest == add_a_b_lowest
-  in
-  // let body (i:size_t { 0 <= v i /\ v i < v aDeg })
-  // : Stack unit
-  //   (requires (fun h -> inv h (v i)))
-  //   (ensures (fun h0 _ h1 -> inv h0 (v i) ))
-  // =
-  //   res.(i) <- add_zq (poly_index a i) (poly_index b i)
-  // in
-  Lib.Loops.for 0ul aDeg inv 
-  (fun i ->
-    // res.(i) <- add_zq (poly_index a i) (poly_index b i)
-    res.(i) <- u32 3328
+    disjoint a b /\ disjoint a res /\ disjoint b res
   )
+  (ensures fun h0 _ h1 ->
+    live h1 a /\ 
+    live h1 b /\ 
+    live h1 res /\
+    disjoint a b /\
+    disjoint a res /\
+    disjoint b res /\
+    modifies (loc res) h0 h1 /\
+    Seq.equal (lpoly_v h1 res) (S.add_rq (lpoly_v h0 a) (lpoly_v h0 b))
+   )
+let add_rq a b res = add #n a b res
+
+val scalar_mul:
+    #deg: size_t
+  -> a:lpoly deg
+  -> b:zq
+  -> res:lpoly deg
+  -> Stack unit
+  (requires fun h ->
+    live h a /\ live h res /\
+    disjoint a res
+  )
+  (ensures fun h0 _ h1 ->
+    live h1 a /\
+    live h1 res /\
+    disjoint a res /\
+    modifies (loc res) h0 h1 /\
+    Seq.equal (lpoly_v h1 res) (S.scalar_mul (lpoly_v h0 a) (zq_v b))
+   )
+
+let scalar_mul #deg a b res =
+  push_frame ();
+  let h0 = ST.get () in
+  let spec_prod: erased _ = S.scalar_mul (lpoly_v h0 a) (zq_v b) in
+  let inv h (i:nat) =
+    live h a /\ live h res /\ modifies (loc res) h0 h /\
+    i <= v deg /\
+    Seq.equal (Seq.slice (lpoly_v h res) 0 i) (Seq.slice spec_prod 0 i) in
+  let body (i: U32.t{ 0 <= U32.v i /\ U32.v i < U32.v deg }):
+    Stack unit
+    (requires (fun h -> inv h (U32.v i)))
+    (ensures (fun h0 () h1 -> inv h0 (U32.v i) /\ inv h1 (U32.v i + 1)))
+    =
+      let h0 = ST.get () in
+      assert (Seq.equal (Seq.slice (lpoly_v h0 res) 0 (v i)) (Seq.slice spec_prod 0 (v i)));
+      let ai = a.(i) in
+      let prod = mul_zq ai b in
+      res.(i) <- prod;
+      let h1 = ST.get () in
+      assert (Seq.equal (Seq.slice (lpoly_v h1 res) 0 (v i)) (Seq.slice spec_prod 0 (v i)));
+      slice_plus_one #_ #(v deg) #(v deg) (lpoly_v h1 res) spec_prod (v i)
+    in
+  Lib.Loops.for 0ul deg inv body;
+  pop_frame ()
+
+val mul:
+    #deg: size_t
+  -> a:lpoly deg
+  -> b:lpoly deg
+  -> res:lpoly deg
+  -> Stack unit
+  (requires fun h ->
+    live h a /\ live h b /\ live h res /\
+    disjoint a b /\ disjoint a res /\ disjoint b res
+  )
+  (ensures fun h0 _ h1 ->
+    live h1 a /\
+    live h1 b /\
+    live h1 res /\
+    disjoint a b /\
+    disjoint a res /\
+    disjoint b res /\
+    modifies (loc res) h0 h1 /\
+    Seq.equal (lpoly_v h1 res) (S.mul (lpoly_v h0 a) (lpoly_v h0 b))
+   )
+
+// let mul #deg a b res =
+//   push_frame ();
+//   let h0 = ST.get () in
+//   let spec_prod: erased _ = S.mul (lpoly_v h0 a) (lpoly_v h0 b) in
+//   let inv h (i:nat) =
+//     live h a /\ live h b /\ live h res /\ modifies (loc res) h0 h /\
+//     i <= v deg /\
+//     Seq.equal (Seq.slice (lpoly_v h res) 0 i) (Seq.slice spec_sum 0 i) in
+//   let body (i: U32.t{ 0 <= U32.v i /\ U32.v i < U32.v deg }):
+//     Stack unit
+//     (requires (fun h -> inv h (U32.v i)))
+//     (ensures (fun h0 () h1 -> inv h0 (U32.v i) /\ inv h1 (U32.v i + 1)))
+//     =
+//       let h0 = ST.get () in
+//       assert (Seq.equal (Seq.slice (lpoly_v h0 res) 0 (v i)) (Seq.slice spec_sum 0 (v i)));
+//       let ai = a.(i) in
+//       let bi = b.(i) in
+//       let sum = add_zq ai bi in
+//       res.(i) <- sum;
+//       let h1 = ST.get () in
+//       assert (Seq.equal (Seq.slice (lpoly_v h1 res) 0 (v i)) (Seq.slice spec_sum 0 (v i)));
+//       assert (Seq.index (lpoly_v h1 res) (v i) == Seq.index spec_sum (v i));
+//       slice_plus_one #_ #(v deg) #(v deg) (lpoly_v h1 res) spec_sum (v i)
+//     in
+//   Lib.Loops.for 0ul deg inv body;
+//   pop_frame () 
